TA_Network/NTA_Temp_Planning_Sem.thy
@@ -2840,6 +2840,15 @@ lemma happ_combine:
   unfolding mutex_snap_def
   by blast+
 
+(* All previous instant actions are happening *)
+
+(* start is happening *)
+
+(* end is happening *)
+
+lemma mutex_commute: undefined
+  using happ_combine unfolding app_effs_def
+
 definition instant_actions_at where
 "instant_actions_at t \<equiv> {a \<in> actions. (t, at_start a) \<in> happ_seq \<and> (t, at_end a) \<in> happ_seq}"
 
